reorganized some mapping properties, added ext map simulation for ordered dynamic semantics

core/PartialExtendedMapSimulations.v
@@ -103,6 +103,15 @@ Class FailMsgParamsPartialExtendedMapCongruency
     pt_ext_fail_msg_fst_snd : pt_ext_map_msg msg_fail = Some (msg_fail)
   }.
 
+Class NewMsgParamsPartialExtendedMapCongruency 
+  (B0 : BaseParams) (B1 : BaseParams)
+  (P0 : MultiParams B0) (P1 : MultiParams B1)
+  (F0 : NewMsgParams P0) (F1 : NewMsgParams P1)
+  (P : MultiParamsPartialExtendedMap P0 P1) :=
+  {
+    pt_ext_new_msg_fst_snd : pt_ext_map_msg msg_new = Some (msg_new)
+  }.
+
 Section PartialExtendedMapSimulations.
 
 Context {base_fst : BaseParams}.
@@ -562,27 +571,6 @@ exists tr'.
 by rewrite /pt_ext_map_onet H_eq H_eq'.
 Qed.
 
-Lemma pt_ext_not_in_failed_not_in :
-  forall n failed,
-    ~ In n failed ->
-    ~ In (tot_map_name n) (map tot_map_name failed).
-Proof.
-move => n.
-elim => //=.
-move => n' failed IH H_in H_in'.
-case: H_in' => H_in'.
-  case: H_in.
-  left.
-  rewrite -(tot_map_name_inv_inverse n').
-  rewrite H_in'.
-  exact: tot_map_name_inv_inverse.
-contradict H_in'.
-apply: IH.
-move => H_in'.
-case: H_in.
-by right.
-Qed.
-
 Lemma pt_ext_map_in_in :
   forall m m0 n l,
   (forall nm, In nm l -> snd nm = m) ->
@@ -692,7 +680,7 @@ case (rel_dec _ _) => H_dec /=.
 exact: IH.
 Qed.
 
-Lemma in_tot_map_name :
+Lemma ext_in_tot_map_name :
 forall m m' l n,
 pt_ext_map_msg m = Some m' ->
 (forall nm, In nm l -> snd nm = m) ->
@@ -729,151 +717,6 @@ by right.
 Qed.
 
 Context {overlay_map_congr : NameOverlayParamsTotalMapCongruency overlay_fst overlay_snd name_map}.
-
-Lemma pt_ext_in_msg_for_adjacent_to :
-  forall (m : @msg _ multi_fst) ns failed h n,
-    In (tot_map_name_inv n, m) (map_pair m (filter_rel h (exclude failed ns))) ->
-    In (tot_map_name_inv n) (filter_rel h (exclude failed ns)).
-Proof.
-move => m.
-elim => //=.
-move => n l IH failed h n'. 
-case (in_dec _ _ _) => H_dec; first exact: IH.
-rewrite /=.
-case (rel_dec _ _) => H_dec' /=.
-  move => H_in.
-  case: H_in => H_in.
-    inversion H_in.
-    by left.
-  right.
-  exact: IH.
-exact: IH.
-Qed.
-
-Lemma pt_ext_in_adjacent_exclude_in_exlude :
-  forall ns failed n h,
-    In (tot_map_name_inv n) (filter_rel h (exclude failed ns)) ->
-    In (tot_map_name_inv n) (exclude failed ns) /\ adjacent_to h (tot_map_name_inv n).
-Proof.
-elim => //=.
-move => n l IH failed n' h.
-case (in_dec _ _ _) => /= H_dec.
-  move => H_in.
-  exact: IH.
-case (rel_dec _ _) => /= H_dec'.
-  move => H_in.
-  case: H_in => H_in.
-    rewrite {1}H_in -{4}H_in.
-    split => //.
-    by left.
-  apply IH in H_in.
-  move: H_in => [H_eq H_in].
-  split => //.
-  by right.
-move => H_in.
-apply IH in H_in.
-move: H_in => [H_eq H_in].
-split => //.
-by right.
-Qed.
-
-Lemma pt_ext_in_failed_exclude :
-  forall ns failed n,
-  In (tot_map_name_inv n) (exclude failed ns) ->
-  ~ In (tot_map_name_inv n) failed /\ In (tot_map_name_inv n) ns.
-Proof.
-elim => //=.
-move => n ns IH failed n'.
-case (in_dec _ _ _) => H_dec /=.
-  move => H_in.
-  apply IH in H_in.
-  move: H_in => [H_in H_in'].
-  split => //.
-  by right.
-move => H_in.
-case: H_in => H_in.
-  rewrite -{1}H_in {2}H_in.
-  split => //.
-  by left.
-apply IH in H_in.
-move: H_in => [H_in H_in'].
-split => //.
-by right.
-Qed.
-
-Lemma pt_ext_in_in_adj_msg_for :
-  forall (m : msg) ns failed n h,
-    In n ns ->
-    ~ In n (map tot_map_name failed) ->
-    adjacent_to h n ->
-    In (n, m)
-     (map_pair m
-        (filter_rel h
-           (exclude (map tot_map_name failed) ns))).
-Proof.
-move => m.
-elim => //=.
-move => n ns IH failed n' h H_in H_in' H_adj.
-case (in_dec _ _ _) => H_dec.
-  case: H_in => H_in; first by rewrite -H_in in H_in'.
-  exact: IH.
-case: H_in => H_in.
-  rewrite H_in.
-  rewrite /=.
-  case (rel_dec _ _) => H_dec' //.
-  rewrite /=.
-  by left.
-rewrite /=.
-case (rel_dec _ _) => H_dec'.
-  rewrite /=.
-  right.
-  exact: IH.
-exact: IH.
-Qed.
-
-Lemma pt_ext_in_exclude_not_in_failed_map :
-  forall ns n failed,
-  In n (exclude (map tot_map_name failed) ns) ->
-  ~ In n (map tot_map_name failed) /\ In n ns.
-Proof.
-elim => //=.
-move => n ns IH n' failed.
-case (in_dec _ _ _) => H_dec.
-  move => H_in.
-  apply IH in H_in.
-  move: H_in => [H_nin H_in].
-  split => //.
-  by right.
-rewrite /=.
-move => H_in.
-case: H_in => H_in.
-  rewrite H_in.
-  rewrite H_in in H_dec.
-  split => //.
-  by left.
-apply IH in H_in.
-move: H_in => [H_nin H_in].
-split => //.
-by right.
-Qed.
-
-Lemma pt_ext_not_in_map_not_in_failed :
-    forall failed n,
-    ~ In n (map tot_map_name failed) ->
-    ~ In (tot_map_name_inv n) failed.
-Proof.
-elim => //=.
-move => n ns IH n' H_in H_in'.
-case: H_in' => H_in'.
-  case: H_in.
-  left.
-  by rewrite H_in' tot_map_name_inverse_inv.
-contradict H_in'.
-apply: IH.
-move => H_in'.
-case: H_in.
-by right.
-Qed.
 
 Lemma in_pt_ext_map_msg_for :
   forall m m' l n,
@@ -915,41 +758,72 @@ apply: H_in.
 by right.
 Qed.
 
-Lemma pt_ext_adjacent_in_in :
-  forall (m : @msg _ multi_fst) ns n h,
-    adjacent_to h (tot_map_name_inv n) ->
-    In (tot_map_name_inv n) ns ->
-    In (tot_map_name_inv n, m) (map_pair m (filter_rel h ns)).
+Lemma pt_ext_nodup_perm_map_map_pair_perm :
+  forall m m' h failed ns ns',
+  NoDup ns ->
+  Permutation (map tot_map_name ns) ns' ->
+  pt_ext_map_msg m = Some m' ->
+  Permutation 
+    (fold_right
+              (fun (nm : name * msg) (l : list (name * msg)) =>
+               match pt_ext_map_msg (snd nm) with
+               | Some m0 => (tot_map_name (fst nm), m0) :: l
+               | None => l
+               end) [] (map_pair m (filter_rel h (exclude failed ns))))
+    (map_pair m' (filter_rel (tot_map_name h) (exclude (map tot_map_name failed) ns'))).
 Proof.
-move => m.
-elim => //=.
-move => n ns IH n' h H_adj H_in.
-case (rel_dec _ _) => H_dec; case: H_in => H_in.
-- rewrite /=.
-  left.
-  by rewrite H_in.
-- rewrite /=.
-  right.
-  exact: IH.
-- by rewrite H_in in H_dec.
-- exact: IH.
-Qed.
-
-Lemma pt_ext_not_in_failed_in_exclude :
-  forall ns n failed,
-  ~ In (tot_map_name_inv n) failed ->
-  In (tot_map_name_inv n) ns ->
-  In (tot_map_name_inv n) (exclude failed ns).
-Proof.
-elim => //=.
-move => n ns IH n' failed H_in H_in'.
-case (in_dec _ _ _) => H_dec; case: H_in' => H_in'.
-- by rewrite H_in' in H_dec.
-- exact: IH.
-- rewrite /=.
-  by left.
-- right.
-  exact: IH.
+move => m m' h failed ns ns' H_nd H_pm H_eq.
+apply NoDup_Permutation; last split.
+- apply (@nodup_pt_ext_map m); first exact: in_for_msg.
+  apply nodup_map_pair.
+  exact: nodup_exclude.
+- apply nodup_map_pair.
+  apply nodup_exclude.
+  move: H_pm.
+  apply: NoDup_Permutation_NoDup.
+  exact: nodup_to_map_name.
+- case: x => n m0 H_in.
+  have H_eq' := pt_ext_map_in_snd _ _ _ _ H_eq H_in.
+  rewrite /= in H_eq'.
+  rewrite H_eq' in H_in.
+  rewrite H_eq' {H_eq' m0}.
+  apply (@ext_in_tot_map_name m) in H_in => //.
+    apply in_map_pair_adjacent_to in H_in.
+    apply in_adjacent_exclude_in_exlude in H_in.
+    move: H_in => [H_in H_adj].
+    apply in_failed_exclude in H_in.
+    move: H_in => [H_in H_in'].
+    have H_nin: ~ In n (map tot_map_name failed).
+      rewrite -(tot_map_name_inverse_inv n).
+      exact: not_in_failed_not_in.
+    apply tot_adjacent_to_fst_snd in H_adj.
+    rewrite tot_map_name_inverse_inv in H_adj.
+    have H_inn: In n ns'.
+      apply (Permutation_in n) in H_pm => //.
+      rewrite -(tot_map_name_inverse_inv n).
+      exact: in_failed_in.
+    exact: in_in_adj_map_pair.
+  exact: in_for_msg.
+- case: x => n m0 H_in.
+  have H_eq' := in_for_msg _ _ _ _ H_in.
+  rewrite /= in H_eq'.
+  rewrite H_eq'.
+  rewrite H_eq' in H_in.
+  apply in_map_pair_related_in in H_in.
+  move: H_in => [H_adj H_in].
+  rewrite -(tot_map_name_inverse_inv n) in H_adj.
+  apply tot_adjacent_to_fst_snd in H_adj.
+  apply in_exclude_not_in_failed_map in H_in.
+  move: H_in => [H_in_f H_in].
+  apply not_in_map_not_in_failed in H_in_f.
+  have H_in_n: In (tot_map_name_inv n) ns.
+    apply Permutation_sym in H_pm.
+    apply (Permutation_in n) in H_pm => //.
+    apply: tot_map_name_in.
+    by rewrite tot_map_name_inverse_inv.
+  apply: (@in_pt_ext_map_msg_for m) => //; first by move => nm; apply in_for_msg.
+  apply adjacent_in_in_msg => //.
+  exact: not_in_failed_in_exclude.
 Qed.
 
 Lemma pt_ext_map_msg_for_eq :
@@ -965,49 +839,9 @@ Lemma pt_ext_map_msg_for_eq :
     (map_pair m' (filter_rel (tot_map_name h) (exclude (map tot_map_name failed) nodes))).
 Proof.
 move => m m' h failed H_eq.
-apply NoDup_Permutation; last split.
-- apply (@nodup_pt_ext_map m); first exact: in_for_msg.
-  apply nodup_map_pair.
-  apply nodup_exclude.
-  exact: no_dup_nodes.
-- apply nodup_map_pair.
-  apply nodup_exclude.
-  exact: no_dup_nodes.
-- case: x => n m0 H_in.
-  have H_eq' := pt_ext_map_in_snd _ _ _ _ H_eq H_in.
-  rewrite /= in H_eq'.
-  rewrite H_eq' in H_in.
-  rewrite H_eq' {H_eq' m0}.
-  apply (@in_tot_map_name m) in H_in => //.
-    apply pt_ext_in_msg_for_adjacent_to in H_in.
-    apply pt_ext_in_adjacent_exclude_in_exlude in H_in.
-    move: H_in => [H_in H_adj].
-    apply pt_ext_in_failed_exclude in H_in.
-    move: H_in => [H_in H_in'].
-    have H_nin: ~ In n (map tot_map_name failed).
-      rewrite -(tot_map_name_inverse_inv n).
-      exact: pt_ext_not_in_failed_not_in.
-    apply tot_adjacent_to_fst_snd in H_adj.
-    rewrite tot_map_name_inverse_inv in H_adj.
-    have H_inn: In n nodes by exact: all_names_nodes.
-    exact: pt_ext_in_in_adj_msg_for.
-  exact: in_for_msg.
-- case: x => n m0 H_in.
-  have H_eq' := in_for_msg _ _ _ _ H_in.
-  rewrite /= in H_eq'.
-  rewrite H_eq'.
-  rewrite H_eq' in H_in.
-  apply in_map_pair_related_in in H_in.
-  move: H_in => [H_adj H_in].
-  rewrite -(tot_map_name_inverse_inv n) in H_adj.
-  apply tot_adjacent_to_fst_snd in H_adj.
-  apply pt_ext_in_exclude_not_in_failed_map in H_in.
-  move: H_in => [H_in_f H_in].
-  apply pt_ext_not_in_map_not_in_failed in H_in_f.
-  have H_in_n: In (tot_map_name_inv n) nodes by exact: all_names_nodes.
-  apply: (@in_pt_ext_map_msg_for m) => //; first by move => nm; apply in_for_msg.
-  apply pt_ext_adjacent_in_in => //.
-  exact: pt_ext_not_in_failed_in_exclude.
+apply pt_ext_nodup_perm_map_map_pair_perm => //; first exact: no_dup_nodes.
+apply Permutation_sym.
+exact: permutation_nodes.
 Qed.
 
 Context {fail_msg_fst : FailMsgParams multi_fst}.
@@ -1031,7 +865,7 @@ invcs H_step.
       case H_m0: (pt_ext_map_msg _) => [m0|]; last by rewrite H_m in H_m0.
       rewrite H_m in H_m0.
       by inversion H_m0.
-    * exact: pt_ext_not_in_failed_not_in.
+    * exact: not_in_failed_not_in.
     * rewrite /= tot_map_name_inv_inverse.
       have H_q := @pt_ext_net_handlers_some _ _ _ _ _ _ multi_map_congr _ _ _ _ _ _ _ _ H_m H_n.
       rewrite /pt_ext_mapped_net_handlers /= in H_q.
@@ -1067,7 +901,7 @@ invcs H_step.
     case H_h: (input_handlers (tot_map_name h) inp' (pt_ext_map_data (onwState net h) h)) => [[out' d'] ps].
     exists [(tot_map_name h, inl inp'); (tot_map_name h, inr out')].
     apply (@SOF_input _ _ _ _ _ _ _ _ _ _ (pt_ext_map_data d h) (pt_ext_map_name_msgs l)).
-    * exact: pt_ext_not_in_failed_not_in.
+    * exact: not_in_failed_not_in.
     * rewrite /= tot_map_name_inv_inverse.
       have H_q := @pt_ext_input_handlers_some _ _ _ _ _ _ multi_map_congr h inp (onwState net h) _ _ _ _ H_i H_h.
       rewrite /pt_ext_mapped_input_handlers /= in H_q.
@@ -1103,7 +937,7 @@ invcs H_step.
     by rewrite (pt_ext_map_in_snd _ _ _ _ pt_ext_fail_msg_fst_snd H_in) (pt_ext_map_in_snd _ _ _ _ pt_ext_fail_msg_fst_snd H_in').
   exists [].
   apply: SOF_fail => //.
-  * exact: pt_ext_not_in_failed_not_in.
+  * exact: not_in_failed_not_in.
   * rewrite /=.
     rewrite /l collate_pt_ext_map_eq /pt_ext_map_name_msgs.
     by rewrite (nodup_perm_collate_eq _ _ H_nd (pt_ext_map_msg_for_eq msg_fail h failed pt_ext_fail_msg_fst_snd)).
@@ -1142,6 +976,252 @@ case: H => H.
   apply: H_trans.
   have ->: tr'' = tr'' ++ [] by rewrite -app_nil_end.
   apply: (@RT1nTStep _ _ _ _ (map tot_map_name failed'', pt_ext_map_onet net'')) => //.
+  exact: RT1nTBase.  
+move: H => [H_eq_n H_eq_f].
+rewrite H_eq_n -H_eq_f.
+move: IHH_step1 => [tr' H_star].
+by exists tr'.
+Qed.
+
+Lemma collate_ls_pt_ext_map_eq :
+  forall ns f h m m',
+    pt_ext_map_msg m = Some m' ->
+    (fun src dst => pt_ext_map_msgs (collate_ls ns f h m (tot_map_name_inv src) (tot_map_name_inv dst))) =
+    collate_ls (map tot_map_name ns) (fun src dst => pt_ext_map_msgs (f (tot_map_name_inv src) (tot_map_name_inv dst))) (tot_map_name h) m'.
+Proof.
+elim => //=.
+move => n ns IH f h m m' H_eq.
+rewrite /= (IH _ _ _  m') //=.
+rewrite 2!tot_map_name_inv_inverse /=.
+set f1 := fun _ _ => _.
+set f2 := update2 _ _ _ _.
+have H_eq_f: f1 = f2.
+  rewrite /f1 /f2 {f1 f2}.
+  have H_eq' := pt_ext_map_msg_update2 f (f n h ++ [m]) h n.
+  rewrite pt_ext_map_msgs_app_distr in H_eq'.
+  by rewrite H_eq' /= H_eq.
+by rewrite H_eq_f.
+Qed.
+
+Context {new_msg_fst : NewMsgParams multi_fst}.
+Context {new_msg_snd : NewMsgParams multi_snd}.
+Context {new_msg_map_congr : NewMsgParamsPartialExtendedMapCongruency new_msg_fst new_msg_snd multi_map}.
+
+Definition pt_ext_map_odnet (net : @ordered_dynamic_network _ multi_fst) : @ordered_dynamic_network _ multi_snd :=
+{| odnwNodes := map tot_map_name net.(odnwNodes) ;
+   odnwPackets := fun src dst => pt_ext_map_msgs (net.(odnwPackets) (tot_map_name_inv src) (tot_map_name_inv dst)) ;
+   odnwState := fun n => match net.(odnwState) (tot_map_name_inv n) with
+                         | None => None
+                         | Some d => Some (pt_ext_map_data d (tot_map_name_inv n))
+                         end |}.
+
+Theorem step_o_d_f_pt_ext_mapped_simulation_1 :
+  forall net net' failed failed' tr,
+    NoDup (odnwNodes net) ->
+    @step_o_d_f _ _ overlay_fst new_msg_fst fail_msg_fst (failed, net) (failed', net') tr ->
+    (exists tr', @step_o_d_f _ _ overlay_snd new_msg_snd fail_msg_snd (map tot_map_name failed, pt_ext_map_odnet net) (map tot_map_name failed', pt_ext_map_odnet net') tr') \/ (pt_ext_map_odnet net' = pt_ext_map_odnet net /\ failed = failed').
+Proof.
+move => net net' failed failed' tr H_nd H_step.
+invcs H_step.
+- left.
+  rewrite /pt_ext_map_odnet.
+  exists [].
+  apply (@SODF_start _ _ _ _ _ _ _ _ (tot_map_name h)) => /=; first exact: not_in_failed_not_in.
+  set p1 := fun _ _ => _.
+  set p2 := collate_ls _ _ _ _.
+  set s1 := fun _ => _.
+  set s2 := update_opt _ _ _.
+  have H_eq_s: s1 = s2.
+    rewrite /s1 /s2 /update_opt {s1 s2}.
+    apply functional_extensionality => n.
+    rewrite -pt_ext_init_handlers_eq.
+    break_match_goal.
+      break_if; break_if; try by congruence.
+      - by repeat find_rewrite; repeat find_rewrite_lem tot_map_name_inv_inverse.
+      - by find_reverse_rewrite; find_rewrite_lem tot_map_name_inverse_inv.
+      - by find_rewrite.
+    break_if; break_if; (try by congruence); last by find_rewrite.
+    by repeat find_rewrite; repeat find_rewrite_lem tot_map_name_inv_inverse.
+  rewrite H_eq_s /s2 {s1 s2 H_eq_s}.
+  have H_eq_p: p1 = p2.
+    rewrite /p1 /p2 {p1 p2}.    
+    rewrite (collate_ls_pt_ext_map_eq _ _ _ _ pt_ext_new_msg_fst_snd) /=.
+    rewrite collate_pt_ext_map_eq.
+    set f1 := fun _ _ => _.    
+    set c1 := collate _ _ _.
+    set c2 := collate _ _ _.
+    set f'1 := map tot_map_name _.
+    set f'2 := filter_rel (tot_map_name h) _.
+    have H_c: c1 = c2.
+      rewrite /c1 /c2 {c1 c2}.
+      apply: nodup_perm_collate_eq; last first.
+        rewrite /pt_ext_map_name_msgs.
+        apply: pt_ext_nodup_perm_map_map_pair_perm => //.
+        by rewrite pt_ext_new_msg_fst_snd.
+      rewrite /pt_ext_map_name_msgs /=.
+      apply: nodup_snd_fst => //.
+        apply (@nodup_pt_ext_map msg_new); first exact: in_for_msg.
+        apply: nodup_map_pair.
+        exact: nodup_exclude.
+      move => nm nm' H_in H_in'.
+      apply (@pt_ext_map_in_snd msg_new _ _ _ _ pt_ext_new_msg_fst_snd) in H_in.
+      apply (@pt_ext_map_in_snd msg_new _ _ _ _ pt_ext_new_msg_fst_snd) in H_in'.
+      by rewrite H_in H_in'.
+    rewrite H_c {H_c}.
+    suff H_suff: f'1 = f'2 by rewrite H_suff.
+    rewrite /f'1 /f'2.
+    elim (odnwNodes net) => //=.
+    move => n ns IH.
+    repeat break_if => //=.
+    * by rewrite IH.
+    * by find_apply_lem_hyp tot_adjacent_to_fst_snd.
+    * by find_apply_lem_hyp not_in_failed_not_in.
+    * by find_apply_lem_hyp tot_adjacent_to_fst_snd.
+    * case: n0.
+      exact: in_failed_in.  
+  by rewrite H_eq_p.
+- case H_m: (pt_ext_map_msg m) => [m'|].
+    left.
+    case H_n: (net_handlers (tot_map_name to) (tot_map_name from) m' (pt_ext_map_data d to)) => [[out' d''] ps].
+    exists [(tot_map_name to, inr out')].
+    rewrite /pt_ext_map_onet /=.
+    apply (@SODF_deliver _ _ _ _ _ _ _ _ m' (pt_ext_map_msgs ms) _ (pt_ext_map_data d to) (pt_ext_map_data d' to) (pt_ext_map_name_msgs l) (tot_map_name from)).
+    * exact: not_in_failed_not_in.
+    * exact: in_failed_in.
+    * by rewrite /= tot_map_name_inv_inverse /= H5.
+    * rewrite /= 2!tot_map_name_inv_inverse /=.
+      find_rewrite.
+      by rewrite /= H_m.
+    * have H_q := @pt_ext_net_handlers_some _ _ _ _ _ _ multi_map_congr _ _ _ _ _ _ _ _ H_m H_n.
+      rewrite /pt_ext_mapped_net_handlers /= in H_q.
+      by repeat break_let; repeat tuple_inversion.
+    * rewrite /= /pt_ext_map_odnet /=.
+      set u1 := fun _ => match _ with | _ => _ end.
+      set u2 := update_opt _ _ _.
+      rewrite collate_pt_ext_map_update2_eq.
+      suff H_suff: u1 = u2 by rewrite H_suff.
+      rewrite /u1 /u2 /update_opt /=.
+      apply functional_extensionality => n.
+      repeat break_if; try by congruence.
+        rewrite -(tot_map_name_inverse_inv n) in n0.
+        by rewrite e in n0.
+      find_rewrite.
+      by find_rewrite_lem tot_map_name_inv_inverse.
+  right.
+  split => //.
+  have [H_eq_d H_ms] := pt_ext_net_handlers_none _ _ _ _ H_m H8.
+  rewrite /pt_ext_map_odnet /= collate_pt_ext_map_update2_eq H_ms /=.
+  set nwP1 := update2 _ _ _ _.
+  set nwS1 := fun _ => match _ with _ => _ end.
+  set nwP2 := fun _ _ => _.
+  set nwS2 := fun _ => _.
+  have H_eq_s: nwS1 = nwS2.
+    rewrite /nwS1 /nwS2 {nwS1 nwS2}.
+    apply functional_extensionality => n.
+    rewrite /update_opt /=.
+    break_if => //.
+    find_rewrite.
+    rewrite H5.
+    by congruence.
+  have H_eq_p: nwP1 = nwP2.
+    rewrite /nwP1 /nwP2 /=.
+    apply functional_extensionality => src.
+    apply functional_extensionality => dst.
+    rewrite /update2 /=.
+    break_if => //.
+    break_and.
+    by rewrite -H -H0 2!tot_map_name_inv_inverse H6 /= H_m.
+  by rewrite H_eq_s H_eq_p.
+- case H_i: (pt_ext_map_input inp h d) => [inp'|].
+    left.
+    case H_h: (input_handlers (tot_map_name h) inp' (pt_ext_map_data d h)) => [[out' d''] ps].
+    exists [(tot_map_name h, inl inp'); (tot_map_name h, inr out')].
+    apply (@SODF_input _ _ _ _ _ _ _ _ _ _ _ (pt_ext_map_data d h) (pt_ext_map_data d' h) (pt_ext_map_name_msgs l)).
+    * exact: not_in_failed_not_in.
+    * exact: in_failed_in. 
+    * by rewrite /pt_ext_map_odnet /= tot_map_name_inv_inverse H5.
+    * have H_q := @pt_ext_input_handlers_some _ _ _ _ _ _ multi_map_congr h inp d _ _ _ _ H_i H_h.
+      rewrite /pt_ext_mapped_input_handlers /= in H_q.
+      rewrite H7 in H_q.
+      by repeat tuple_inversion.
+    * rewrite /= /pt_ext_map_odnet /= collate_pt_ext_map_eq.
+      set u1 := fun _ => match _ with | _ => _ end.
+      set u2 := update_opt _ _ _.
+      suff H_suff: u1 = u2 by rewrite H_suff.
+      rewrite /u1 /u2 /update_opt /=.
+      apply functional_extensionality => n.
+      repeat break_if; try by congruence.
+        rewrite -(tot_map_name_inverse_inv n) in n0.
+        by rewrite e in n0.
+      find_rewrite.
+      by find_rewrite_lem tot_map_name_inv_inverse.
+  right.
+  rewrite /= /pt_ext_map_odnet /=.
+  have [H_d H_l] := pt_ext_input_handlers_none h inp d H_i H7.
+  split => //=.
+  rewrite collate_pt_ext_map_eq H_l /=.
+  set nwS1 := fun n : name => match _ with | _ => _ end.
+  set nwS2 := fun n : name => match _ with | _ => _ end.
+  have H_eq_n: nwS1 = nwS2.
+    rewrite /nwS1 /nwS2 /=.
+    apply functional_extensionality => n.
+    rewrite /update_opt /=.
+    break_if => //.
+    by repeat find_rewrite.
+  by rewrite H_eq_n.
+- left.
+  rewrite /pt_ext_map_odnet /=.
+  set l := map_pair _ _.
+  have H_nd': NoDup (map (fun nm => fst nm) (pt_ext_map_name_msgs l)).
+    rewrite /pt_ext_map_name_msgs /=.
+    rewrite /l {l}.
+    apply nodup_snd_fst.
+      apply (@nodup_pt_ext_map msg_fail); first exact: in_for_msg.
+      apply nodup_map_pair.
+      exact: nodup_exclude.
+    move => nm nm' H_in H_in'.
+    by rewrite (pt_ext_map_in_snd  _ _ _ _ pt_ext_fail_msg_fst_snd H_in) (pt_ext_map_in_snd _ _ _ _ pt_ext_fail_msg_fst_snd H_in').
+  exists [].
+  apply: SODF_fail => //.
+  * exact: not_in_failed_not_in.
+  * exact: in_failed_in.
+  * rewrite /=.
+    rewrite /l collate_pt_ext_map_eq.
+    have H_pm := pt_ext_nodup_perm_map_map_pair_perm _ h failed H_nd (Permutation_refl (map tot_map_name (odnwNodes net))) pt_ext_fail_msg_fst_snd.
+    have H_pm' := H_pm _ _ fail_msg_map_congr.
+    have H_eq := nodup_perm_collate_eq  _ _ H_nd' H_pm'.
+    by rewrite H_eq.
+Qed.
+
+Corollary step_o_d_f_pt_mapped_simulation_star_1 :
+  forall net failed tr,
+    @step_o_d_f_star _ _ overlay_fst new_msg_fst fail_msg_fst step_o_d_f_init (failed, net) tr ->
+    exists tr', @step_o_d_f_star _ _ overlay_snd new_msg_snd fail_msg_snd step_o_d_f_init (map tot_map_name failed, pt_ext_map_odnet net) tr'.
+Proof.
+move => net failed tr H_step.
+remember step_o_d_f_init as y in *.
+change failed with (fst (failed, net)).
+change net with (snd (failed, net)) at 2.
+move: Heqy.
+induction H_step using refl_trans_1n_trace_n1_ind => H_init /=.
+  rewrite H_init /step_o_d_f_init /= /step_o_init.
+  exists [].
+  exact: RT1nTBase.
+concludes.
+rewrite H_init {H_init x} in H_step2 H_step1.
+case: x' H IHH_step1 H_step1 => failed' net'.
+case: x'' H_step2 => failed'' net''.
+rewrite /=.
+move => H_step2 H IHH_step1 H_step1.
+find_apply_lem_hyp step_o_d_f_pt_ext_mapped_simulation_1; last by move: H_step1; apply: ordered_dynamic_nodes_no_dup.
+case: H => H.
+  move: IHH_step1 => [tr' H_star].
+  move: H => [tr'' H].
+  exists (tr' ++ tr'').
+  have H_trans := refl_trans_1n_trace_trans H_star.
+  apply: H_trans.
+  have ->: tr'' = tr'' ++ [] by rewrite -app_nil_end.
+  apply: (@RT1nTStep _ _ _ _ (map tot_map_name failed'', pt_ext_map_odnet net'')) => //.
   exact: RT1nTBase.  
 move: H => [H_eq_n H_eq_f].
 rewrite H_eq_n -H_eq_f.
